cfrontend/Cshmgenproof.v
@@ -658,8 +658,8 @@ Proof.
   econstructor. eauto. econstructor. eauto. constructor. 
   econstructor; eauto. 
   apply alignof_blockcopy_1248.
-  apply sizeof_pos. 
-  eapply Zdivide_trans. apply alignof_blockcopy_divides. apply sizeof_alignof_compat.
+  apply sizeof_pos.
+  apply sizeof_alignof_blockcopy_compat.
 Qed.
  
 Lemma make_store_correct:
